Started working on high-level design of Merkle trees

secure_api/merkle_tree/MerkleTree.New.High.fst
@@ -1,13 +1,10 @@
 module MerkleTree.New.High
 
 open EverCrypt
-// open EverCrypt.Hash
 open EverCrypt.Helpers
 
 open FStar.All
 open FStar.Ghost
-open FStar.Integers
-open FStar.Mul
 open FStar.Seq
 
 module List = FStar.List.Tot
@@ -24,8 +21,11 @@ module EHL = EverCrypt.Helpers
 val hash_size: uint32_t
 let hash_size = 32ul
 
-let hash = b:EHS.bytes{S.length b = U32.v hash_size}
-let hash_seq = S.seq hash
+type hash = b:EHS.bytes{S.length b = U32.v hash_size}
+type hash_seq = S.seq hash
+type hash_ss = S.seq hash_seq
+
+let hash_init: hash = S.create (U32.v hash_size) 0uy
 
 val hash_2: src1:hash -> src2:hash -> GTot hash
 let hash_2 src1 src2 =
@@ -33,9 +33,131 @@ let hash_2 src1 src2 =
 
 /// High-level Merkle tree data structure
 
+let merkle_tree_size_lg = 32
+
 noeq type merkle_tree =
-| MT: i:nat -> j:nat{j > i} ->
+| MT: i:nat -> j:nat{j >= i && j < pow2 merkle_tree_size_lg} ->
       hs:S.seq hash_seq{S.length hs = 32} ->
       rhs_ok:bool -> rhs:hash_seq{S.length rhs = 32} ->
       merkle_tree
+
+val mt_not_full: merkle_tree -> GTot bool
+let mt_not_full mt =
+  MT?.j mt < pow2 merkle_tree_size_lg - 1
+
+/// Well-formedness
+
+val offset_of: i:nat -> Tot nat
+let offset_of i =
+  if i % 2 = 0 then i else i - 1
+
+val mt_wf_elts:
+  lv:nat{lv <= 32} ->
+  hs:hash_ss{S.length hs = 32} ->
+  i:nat -> j:nat{j >= i} ->
+  GTot Type0 (decreases (32 - lv))
+let rec mt_wf_elts lv hs i j =
+  if lv = 32 then true
+  else (let ofs = offset_of i in
+       S.length (S.index hs lv) == j - ofs /\
+       mt_wf_elts (lv + 1) hs (i / 2) (j / 2))
+
+val mt_wf: merkle_tree -> GTot Type0
+let mt_wf mt =
+  mt_wf_elts 0 (MT?.hs mt) (MT?.i mt) (MT?.j mt)
+
+type wf_mt = mt:merkle_tree{mt_wf mt}
+
+/// Construction
+
+// NOTE: the public function is `create_mt` defined below, which
+// builds a tree with an initial hash.
+private val create_empty_mt: unit -> GTot wf_mt
+private let create_empty_mt _ =
+  admit ();
+  MT 0 0 (S.create 32 S.empty) false (S.create 32 hash_init)
+
+/// Insertion
+
+private val insert_:
+  lv:nat{lv < 32} ->
+  i:Ghost.erased nat ->
+  j:nat{Ghost.reveal i <= j} ->
+  hs:hash_ss{
+    S.length hs = 32 /\ 
+    mt_wf_elts lv hs (Ghost.reveal i) j} ->
+  acc:hash ->
+  GTot (ihs:hash_ss{
+    S.length ihs = 32 /\
+    mt_wf_elts lv ihs (Ghost.reveal i) (j + 1)})
+  (decreases j)
+private let rec insert_ lv i j hs acc =
+  admit ();
+  let ihs = S.upd hs lv (S.snoc (S.index hs lv) acc) in
+  if j % 2 = 1 && S.length (S.index hs lv) > 0 
+  then (let nacc = hash_2 (S.last (S.index hs lv)) acc in
+       insert_ (lv + 1) 
+	       (Ghost.hide (Ghost.reveal i / 2)) (j / 2)
+	       ihs nacc)
+  else ihs
+
+val mt_insert:
+  mt:wf_mt{mt_not_full mt} -> v:hash -> GTot wf_mt
+let mt_insert mt v =
+  MT (MT?.i mt)
+     (MT?.j mt + 1)
+     (insert_ 0 (Ghost.hide (MT?.i mt)) (MT?.j mt) (MT?.hs mt) v)
+     false
+     (MT?.rhs mt)
+
+val create_mt: init:hash -> GTot wf_mt
+let create_mt init =
+  mt_insert (create_empty_mt ()) init
+
+/// Getting the Merkle root and path
+
+type path = S.seq hash
+
+// Construct the rightmost hashes for a given (incomplete) Merkle tree.
+// This function calculates the Merkle root as well, which is the final
+// accumulator value.
+private val construct_rhs:
+  lv:nat{lv <= 32} ->
+  hs:hash_ss{S.length hs = 32} ->
+  rhs:hash_seq{S.length rhs = 32} ->
+  i:nat ->
+  j:nat{
+    i <= j && j < pow2 (32 - lv) /\
+    mt_wf_elts lv hs i j} ->
+  acc:hash ->
+  actd:bool ->
+  GTot (crhs:hash_seq{S.length crhs = 32} * hash) (decreases j)
+private let rec construct_rhs lv hs rhs i j acc actd =
+  admit ();
+  let ofs = offset_of i in
+  if j = 0 then (rhs, acc)
+  else
+    (if j % 2 = 0
+    then construct_rhs (lv + 1) hs rhs (i / 2) (j / 2) acc actd
+    else (if actd
+    	 then (let nrhs = S.upd rhs lv acc in
+	      let nacc = hash_2 (S.index (S.index hs lv) (j - 1 - ofs)) acc in
+	      construct_rhs (lv + 1) hs nrhs (i / 2) (j / 2) nacc true)
+	 else (let nacc = S.index (S.index hs lv) (j - 1 - ofs) in
+	      construct_rhs (lv + 1) hs rhs (i / 2) (j / 2) nacc true)))
+
+val mt_get_root: mt:wf_mt -> GTot hash
+let mt_get_root mt =
+  let (_, root) = construct_rhs
+		    0 (MT?.hs mt) (MT?.rhs mt) (MT?.i mt) (MT?.j mt)
+		    hash_init false in
+  root
+
+// TODOs:
+// path_insert
+// mt_get_path
+// mt_flush_to
+// mt_flush
+// mt_verify
+
 
